Add VC generation tactic.

Strata/Languages/Boogie/MetaVerifier.lean
@@ -34,10 +34,10 @@ deriving instance ToExpr for Boogie.SMT.Sort
 deriving instance ToExpr for Boogie.SMT.IF
 deriving instance ToExpr for Boogie.SMT.Context
 
-def createGoal (ctx : Boogie.SMT.Context) (terms : List SMT.Term) (name : String) : MetaM MVarId := do
-  let t :: ts := terms | throwError "No terms to discharge"
-  let (ts, t) := ((t :: ts).dropLast, (t :: ts).getLast?.get rfl)
-  let t := Factory.not t
+abbrev SMTVC := String × Boogie.SMT.Context × List Term × Term
+abbrev SMTVCs := List SMTVC
+
+def createGoal : SMTVC → MetaM MVarId := fun (label, ctx, ts, t) => do
   match translateQuery ctx ts.toArray t with
   | .error e =>
     throwError e
@@ -50,50 +50,27 @@ def createGoal (ctx : Boogie.SMT.Context) (terms : List SMT.Term) (name : String
     let oe := mkApp2 (.const ``Option.some [0]) (.sort 0) e
     if !(← Meta.approxDefEq <| Meta.isDefEqGuarded denotation oe) then
       trace[strata.verify] "Warning: denotation does not match generated expression"
-    let .mvar mv ← Meta.mkFreshExprMVar e (userName := Translate.symbolToName name) | throwError "Failed to create goal"
+    let .mvar mv ← Meta.mkFreshExprMVar e (userName := Translate.symbolToName label) | throwError "Failed to create goal"
     return mv
 
 end Strata.SMT
 
 namespace Boogie
 
-def genVCsSingleENV (pE : Program × Env) : MetaM (List MVarId) := do
-  let (p, E) := pE
-  match E.error with
-  | some err =>
-    throwError s!"[Strata.Boogie] Error during evaluation!\n\
-                  {format err}\n\n\
-                  Evaluated program: {p}\n\n"
-  | _ =>
-    let mut mvs := []
-    for obligation in E.deferred do
-      let maybeTerms := ProofObligation.toSMTTerms E obligation
-      match maybeTerms with
-      | .error err =>
-        throwError "[Error] SMT Encoding error for obligation {format obligation.label}: \n\
-                    {err}\n\n\
-                    Evaluated program: {p}\n\n"
-      | .ok (terms, ctx) =>
-        try
-          let mv ← createGoal ctx terms obligation.label
-          mvs := mv :: mvs
-        catch e =>
-           let prog := m!"\n\nEvaluated program:\n{p}"
-           throwError "\n\nObligation {obligation.label}: solver error!\
-                       \n\nError: {e.toMessageData}\
-                       {prog}"
-           break
-    return mvs
+abbrev BoogieVC := Env × Imperative.ProofObligation Expression
+abbrev BoogieVCs := List (Env × Imperative.ProofObligation Expression)
 
-def genVCs (program : Program) (options : Options := Options.default) : MetaM (List MVarId) := do
+def genVCsSingleENV (pE : Program × Env) : Option BoogieVCs := do
+  let (_, E) := pE
+  match E.error with
+  | some _ => none
+  | _ => return E.deferred.toList.map (fun ob => (E, ob))
+
+def genVCs (program : Program) (options : Options := Options.default) : Option BoogieVCs := do
   match Boogie.typeCheckAndPartialEval options program with
-  | .error err =>
-    throwError m!"[Strata.Boogie] Type checking error: {err}"
+  | .error _ => none
   | .ok pEs =>
-    let VCss ← if options.checkOnly then
-                 pure []
-               else
-                 (List.mapM (fun pE => genVCsSingleENV pE) pEs)
+    let VCss ← List.mapM (fun pE => genVCsSingleENV pE) pEs
     return VCss.flatten.reverse
 
 end Boogie
@@ -102,54 +79,324 @@ namespace C_Simp
 
 open C_Simp
 
-def genVCs (program : Strata.C_Simp.Program) (options : Options := Options.default) : MetaM (List MVarId) := do
+def genVCs (program : Strata.C_Simp.Program) (options : Options := Options.default) : Option Boogie.BoogieVCs := do
   let program := Strata.to_boogie program
   Boogie.genVCs program options
 
 end C_Simp
 
-def genVCs (program : Strata.Program) (options : Options := Options.default) : MetaM (List MVarId) := do
+namespace Strata
+
+def genBoogieVCs (program : Program) : Option Boogie.BoogieVCs := do
   if program.dialect == "Boogie" then
-    let (program, errors) := Strata.TransM.run (Strata.translateProgram program)
-    let #[] := errors | throwError s!"DDM Transform Error: {errors}"
-    trace[strata.verify] f!"AST: {program}"
-    Boogie.genVCs program options
+    let (program, #[]) := TransM.run (translateProgram program) | none
+    Boogie.genVCs program { (default : Options) with verbose := false : Options }
   else if program.dialect == "C_Simp" then
-    let (program, errors) := Strata.C_Simp.TransM.run (Strata.C_Simp.translateProgram (program.commands))
-    let #[] := errors | throwError s!"DDM Transform Error: {errors}"
-    trace[strata.verify] f!"AST: {program}"
-    C_Simp.genVCs program options
+    let (program, #[]) := C_Simp.TransM.run (C_Simp.translateProgram (program.commands)) | none
+    C_Simp.genVCs program { (default : Options) with verbose := false : Options }
   else
-    throwError "Unsupported dialect"
+    none
 
-syntax (name := prove_vcs)  "#prove_vcs " ident " by " tacticSeq : command
+def Boogie.ProofObligation.toSMTObligation (E : Boogie.Env) (ob : Imperative.ProofObligation Boogie.Expression) :
+  Option SMT.SMTVC := do
+    let maybeTerms := Boogie.ProofObligation.toSMTTerms E ob
+    match maybeTerms with
+    | .error _ => none
+    | .ok (terms, ctx) =>
+        let t :: ts := terms | none
+        let (ts, t) := ((t :: ts).dropLast, (t :: ts).getLast?.get rfl)
+        let t := SMT.Factory.not t
+        (ob.label, ctx, ts, t)
 
-open Lean.Elab Command in
-@[command_elab prove_vcs] unsafe def elabProveVCs : CommandElab := fun stx => do
+def denoteProofObligation (E : Boogie.Env) (ob : Imperative.ProofObligation Boogie.Expression) :
+  Option Prop := do
+  sorry
+
+theorem DPO_isSome_of_DQ_isSome :
+    (Boogie.ProofObligation.toSMTObligation E ob) = some (label, ctx, ts, t) →
+    (denoteQuery ctx ts t).isSome → (denoteProofObligation E ob).isSome := by
+  sorry
+
+theorem DPO_of_DQ :
+    Boogie.ProofObligation.toSMTObligation E ob = some (label, ctx, ts, t) →
+    denoteQuery ctx ts t = some p → denoteProofObligation E ob = some q →
+    p → q := by
+  sorry
+
+def denoteProofObligations (vcs : Boogie.BoogieVCs) : Option Prop := do
+  match vcs with
+  | [] => return True
+  | (E, ob) :: vcs =>
+    let p ← denoteProofObligation E ob
+    go vcs p
+where
+  go vcs p : Option Prop := do
+  match vcs with
+  | [] => return p
+  | (E, ob) :: vcs =>
+    let q ← denoteProofObligation E ob
+    go vcs (p ∧ q)
+
+def boogieVCsCorrect (program : Program) : Prop :=
+  match genBoogieVCs program with
+  | some vcs => (denoteProofObligations vcs).getD False
+  | none     => False
+
+noncomputable def denoteQueries (vcs : SMT.SMTVCs) : Option Prop := do
+  match vcs with
+  | [] => return True
+  | (_, ctx, ts, t) :: vcs =>
+    let p ← denoteQuery ctx ts t
+    go vcs p
+where
+  go vcs p : Option Prop := do
+  match vcs with
+  | [] => return p
+  | (_, ctx, ts, t) :: vcs =>
+    let q ← denoteQuery ctx ts t
+    go vcs (p ∧ q)
+
+def toSMTVCs vcs := do
+  match vcs with
+  | [] => return []
+  | (E, ob) :: vcs =>
+    let (ctx, ts, t) ← Boogie.ProofObligation.toSMTObligation E ob
+    let vcs ← toSMTVCs vcs
+    return (ctx, ts, t) :: vcs
+
+def genSMTVCs (program : Program) : Option SMT.SMTVCs := do
+  let boogieVCs ← genBoogieVCs program
+  toSMTVCs boogieVCs
+
+def smtVCsCorrect (program : Program) : Prop :=
+  match genSMTVCs program with
+  | some vcs => (denoteQueries vcs).getD False
+  | none     => False
+
+theorem toSMTVCs_cons :
+    toSMTVCs ((E, ob) :: boogieVCs) = some vcs →
+    ∃ label ctx ts t smtVCs, vcs = (label, ctx, ts, t) :: smtVCs ∧
+    Boogie.ProofObligation.toSMTObligation E ob = some (label, ctx, ts, t) ∧
+    toSMTVCs boogieVCs = some smtVCs := by
+  simp only [toSMTVCs, Option.bind_eq_bind, Option.bind]
+  grind
+
+theorem DPOsGo_isSome_of_DQsGo_isSome  :
+    toSMTVCs boogieVCs = some smtVCs → (denoteQueries.go smtVCs p).isSome →
+    (denoteProofObligations.go boogieVCs q).isSome := by
+  intro h hs
+  induction boogieVCs generalizing smtVCs p q with
+  | nil => rfl
+  | cons boogieVC boogieVCs ih =>
+    let (E, ob) := boogieVC
+    let ⟨_, ctx, ts, t, smtVCs, hctx, hob, hrest⟩ := toSMTVCs_cons h
+    simp only [hctx, Option.bind, denoteQueries.go, Option.bind_eq_bind] at hs
+    match hp' : denoteQuery ctx ts t with
+    | none => simp_all
+    | some p' =>
+      simp only [hp'] at hs
+      simp only [denoteProofObligations.go, Option.bind_eq_bind, Option.bind]
+      split
+      · have := DPO_isSome_of_DQ_isSome hob (Option.isSome_of_eq_some hp')
+        simp_all
+      · simp [ih hrest hs]
+
+theorem DPOs_isSome_of_DQs_isSome  :
+    toSMTVCs boogieVCs = some smtVCs → (denoteQueries smtVCs).isSome →
+    (denoteProofObligations boogieVCs).isSome := by
+  intro h hs
+  match boogieVCs with
+  | [] => rfl
+  | (E, ob) :: boogieVCs =>
+    have ⟨_, ctx, ts, t, smtVCs, hctx, hob, hrest⟩ := toSMTVCs_cons h
+    simp only [denoteQueries, hctx, Option.bind_eq_bind, Option.bind] at hs
+    match hp : denoteQuery ctx ts t with
+    | none => simp_all
+    | some p =>
+      simp only [hp] at hs
+      simp only [denoteProofObligations, Option.bind_eq_bind, Option.bind]
+      split
+      · have := DPO_isSome_of_DQ_isSome hob (Option.isSome_of_eq_some hp)
+        simp_all
+      · simp [DPOsGo_isSome_of_DQsGo_isSome hrest hs]
+
+theorem DPOsGo_of_DQsGo  :
+    toSMTVCs boogieVCs = some smtVCs →
+    denoteQueries.go smtVCs p = some P →
+    denoteProofObligations.go boogieVCs q = some Q →
+    (p → q) → P → Q := by
+  intro h
+  induction boogieVCs generalizing smtVCs p q P Q with
+  | nil => simp_all [denoteProofObligations.go, denoteQueries.go, toSMTVCs]
+  | cons boogieVC boogieVCs ih =>
+    let (E, ob) := boogieVC
+    let ⟨_, ctx, ts, t, smtVCs, hctx, hob, hrest⟩ := toSMTVCs_cons h
+    simp only [hctx] at h ⊢
+    simp only [denoteQueries.go, Option.bind_eq_bind, denoteProofObligations.go]
+    match hp' : denoteQuery ctx ts t with
+    | none => simp_all
+    | some p' =>
+      match hq' : denoteProofObligation E ob with
+      | none => simp_all
+      | some q' =>
+        simp only [Option.bind_some]
+        intro hp hq hpq
+        have hp'q' := DPO_of_DQ hob hp' hq'
+        have hpp'qq' : p ∧ p' → q ∧ q' := fun ⟨hp, hp'⟩ => And.intro (hpq hp) (hp'q' hp')
+        apply ih hrest hp hq hpp'qq'
+
+theorem DPOs_of_DQs  :
+    toSMTVCs boogieVCs = some smtVCs →
+    denoteQueries smtVCs = some P →
+    denoteProofObligations boogieVCs = some Q →
+    P → Q := by
+  intro h
+  match boogieVCs with
+  | [] => simp_all [denoteProofObligations, denoteQueries, toSMTVCs]
+  | (E, ob) :: boogieVCs =>
+    have ⟨_, ctx, ts, t, smtVCs, hctx, hob, hrest⟩ := toSMTVCs_cons h
+    simp only [denoteQueries, denoteProofObligations, hctx] at h ⊢
+    match hp : denoteQuery ctx ts t with
+    | none => simp_all
+    | some p =>
+      match hq : denoteProofObligation E ob with
+      | none => simp_all
+      | some q =>
+        simp only [Option.bind_some, Option.bind_eq_bind]
+        intro hP hQ
+        have hpq := DPO_of_DQ hob hp hq
+        apply DPOsGo_of_DQsGo hrest hP hQ hpq
+
+theorem boogieVCsCorrect_of_smtVCsCorrect (program : Program) :
+    smtVCsCorrect program → boogieVCsCorrect program := by
+  simp only [boogieVCsCorrect, smtVCsCorrect, genSMTVCs]
+  match hb : genBoogieVCs program with
+  | none => simp_all
+  | some boogieVCs =>
+    simp only [Option.bind_eq_bind, Option.bind_some]
+    match hs : toSMTVCs boogieVCs with
+    | none => simp_all
+    | some smtVCs =>
+      match hP : denoteQueries smtVCs with
+      | none => simp_all
+      | some P =>
+        match hQ : denoteProofObligations boogieVCs with
+        | none =>
+          have := DPOs_isSome_of_DQs_isSome hs (Option.isSome_of_eq_some hP)
+          simp_all
+        | some Q =>
+          simp only [hP, Option.getD_some]
+          exact DPOs_of_DQs hs hP hQ
+
+namespace Meta
+
+def andN (ps : List Lean.Expr) : Lean.Expr :=
+  match ps with
+  | [] => .const ``True []
+  | p :: ps => go ps p
+where
+  go ps P : Lean.Expr :=
+  match ps with
+  | [] => P
+  | p :: ps => go ps (mkApp2 (.const ``And []) P p)
+
+def andNIntro (hps : List (Lean.Expr × Lean.Expr)) : Lean.Expr :=
+  match hps with
+  | [] => .const ``True.intro []
+  | (p, hp) :: ps => go ps p hp
+where
+  go ps P hP : Lean.Expr :=
+  match ps with
+  | [] => hP
+  | (p, hp) :: ps => go ps (mkApp2 (.const ``And []) P p) (mkApp4 (.const ``And.intro []) P p hP hp)
+
+def nativeDecide (p : Lean.Expr) : MetaM Lean.Expr := do
+  let hp ← Meta.synthInstance (.app (.const ``Decidable []) p)
+  let auxDeclName ← mkNativeAuxDecl `_genSMTVCs (.const ``Bool []) (mkApp2 (.const ``decide []) p hp)
+  let b := .const auxDeclName []
+  return mkApp3 (.const ``of_decide_eq_true []) p hp
+                (mkApp3 (.const ``Lean.ofReduceBool []) b (.const ``true [])
+                        (mkApp2 (.const ``Eq.refl [1]) (.const ``Bool []) (.const ``true [])))
+where
+  mkNativeAuxDecl (baseName : Name) (type value : Lean.Expr) : MetaM Name := do
+    let auxName ← Lean.mkAuxDeclName baseName
+    let decl := Declaration.defnDecl {
+      name := auxName, levelParams := [], type, value
+      hints := .abbrev
+      safety := .safe
+    }
+    addAndCompile decl
+    pure auxName
+
+unsafe def genSMTVCs (mv : MVarId) : MetaM (List MVarId) := do
+  let type ← mv.getType
+  let some program := type.app1? ``Strata.smtVCsCorrect | throwError "Expected a Strata.smtVCsCorrect goal"
+  logInfo m!"Generating SMT VCs for {program}"
+  let mv ← Meta.unfoldTarget mv ``Strata.smtVCsCorrect
+  let ovcs := .app (.const ``Strata.genSMTVCs []) program
+  let ovcsType := .app (.const ``Option [0]) (.const ``Strata.SMT.SMTVCs [])
+  let some evcs ← Meta.evalExpr (Option Strata.SMT.SMTVCs) ovcsType ovcs
+    | throwError "Failed to generate VCs"
+  logInfo m!"Generated {repr evcs}"
+  let eqVCs := mkApp3 (.const ``Eq [1]) ovcsType ovcs (toExpr (some evcs))
+  -- let hEQVCs := mkApp2 (.const ``Eq.refl [1]) ovcsType (toExpr (some evcs))
+  let hEQVCs ← nativeDecide eqVCs
+  let r ← mv.rewrite (← mv.getType) hEQVCs
+  let mv ← mv.replaceTargetEq r.eNew r.eqProof
+  let mvs ← evcs.mapM SMT.createGoal
+  let ps ← mvs.mapM MVarId.getType
+  let hP := andNIntro (List.zip ps (mvs.map Expr.mvar))
+  mv.assign hP
+  return mvs
+
+-- unsafe def genBoogieVCs (mv : MVarId) : MetaM (List MVarId) := do
+--   let type ← mv.getType
+--   let some program := type.app1? ``Strata.boogieVCsCorrect | throwError "Expected a Strata.boogieVCsCorrect goal"
+--   logInfo m!"Generating Boogie VCs for {program}"
+--   let mv ← Meta.unfoldTarget mv ``Strata.boogieVCsCorrect
+--   let ovcs := .app (.const ``Strata.genBoogieVCs []) program
+--   let ovcsType := .app (.const ``Option [0]) (.const ``Boogie.BoogieVCs [])
+--   let some evcs ← Meta.evalExpr (Option Boogie.BoogieVCs) ovcsType ovcs
+--     | throwError "Failed to generate VCs"
+--   logInfo m!"Generated Boogie VCs"
+--   let eqVCs := mkApp3 (.const ``Eq [1]) ovcsType ovcs (toExpr (some evcs))
+--   -- let hEQVCs := mkApp2 (.const ``Eq.refl [1]) ovcsType (toExpr (some evcs))
+--   let hEQVCs ← nativeDecide eqVCs
+--   let r ← mv.rewrite (← mv.getType) hEQVCs
+--   let mv ← mv.replaceTargetEq r.eNew r.eqProof
+--   let mvs ← evcs.mapM SMT.createGoal
+--   let ps ← mvs.mapM MVarId.getType
+--   let hP := andNIntro (List.zip ps (mvs.map Expr.mvar))
+--   mv.assign hP
+--   return mvs
+
+end Meta
+
+namespace Tactic
+
+syntax (name := genSMTVCs) "gen_smt_vcs" : tactic
+
+open Lean Elab Tactic in
+@[tactic genSMTVCs] unsafe def evalGenSMTVCs : Tactic := fun stx => do
   match stx with
-  | `(#prove_vcs $name:ident by $tacs) => liftTermElabM do
-    let type := Expr.const ``Strata.Program []
-    let Expr.const c [] ← Term.elabTerm name type | throwError "Expected a constant"
-    let env ← evalConst Strata.Program c
-    let mvs ← genVCs env { (default : Options) with verbose := false : Options }
-    let ts ← mvs.mapM (liftM ∘ MVarId.getType)
-    let t :: ts := ts | throwError "Expected at least one VC"
-    let (ts, t) := ((t :: ts).dropLast, (t :: ts).getLast?.get rfl)
-    let conj := ts.foldr (mkApp2 (.const ``And [])) t
-    let hconj ← Meta.mkFreshExprMVar conj (userName := c ++ `vcs)
-    let vcs := mvs.map Expr.mvar
-    let vc :: vcs := vcs | throwError "Expected at least one VC"
-    let (vcs, vc) := ((vc :: vcs).dropLast, (vc :: vcs).getLast?.get rfl)
-    let (_, hconjp) := (ts.zip vcs).foldr (init := (t, vc)) fun (t, vc) (ts, vcs) =>
-       (mkApp2 (.const ``And []) t ts, mkApp4 (.const ``And.intro []) t ts vc vcs)
-    let k := do
-      hconj.mvarId!.assign hconjp
-      Tactic.replaceMainGoal mvs
-      Tactic.evalTactic tacs.raw
-      Tactic.pruneSolvedGoals
-    let goals ← Tactic.run hconj.mvarId! k
-    match goals with
-    | [] => return
-    | goals => do
-      throwErrorAt stx m!"Following goals remain {goals.foldl (init := "") (fun acc g => acc ++ m!"\n  {g}")}"
+  | `(tactic| gen_smt_vcs) =>
+    let mvs ← Meta.genSMTVCs (← Tactic.getMainGoal)
+    Tactic.replaceMainGoal mvs
   | _ => throwUnsupportedSyntax
+
+syntax (name := genBoogieVCs) "gen_boogie_vcs" : tactic
+
+open Lean Elab Tactic in
+@[tactic genBoogieVCs] unsafe def evalGenBoogieVCs : Tactic := fun stx => do
+  match stx with
+  | `(tactic| gen_boogie_vcs) =>
+    let mvs ← Meta.genSMTVCs (← Tactic.getMainGoal)
+    Tactic.replaceMainGoal mvs
+  | _ => throwUnsupportedSyntax
+
+end Tactic
+
+end Strata
+
+initialize
+  registerTraceClass `strata.verify
